\begin{align}
\frac{1}{\sqrt{-g}} \frac{\delta S}{\delta \Phi} &= C_{\Phi \Phi} \Phi^2+ C_{\Phi \Psi} \Phi \Psi+ C_{\Phi \pi} \Phi \pi +C_{\Phi \dot{\Phi}} \Phi \dot{\Phi}+ C_{\Phi \dot{\Psi}} \Phi \dot{\Psi}+ C_{\Phi \dot{\pi}} \Phi \dot{\pi}  -\frac{k^2}{C^2} C^{(2)}_{\Phi \Phi} \Phi \Phi  -\frac{k^2}{C^2} C^{(2)}_{\Phi \Psi} \Phi \Psi   -\frac{k^2}{C^2} C^{(2)}_{\Phi \pi} \Phi \pi 
 \nonumber \\ &
 +C_{\Psi \Psi} \Psi \Psi+ C_{\Psi \pi} \Psi \pi +C_{\Psi \dot{\Phi}} \Psi \dot{\Phi}+ C_{\Psi \dot{\Psi}} \Psi \dot{\Psi}+ C_{\Psi \dot{\pi}} \Psi \dot{\pi}  -\frac{k^2}{C^2} C^{(2)}_{\Psi \Phi} \Psi \Phi  -\frac{k^2}{C^2} C^{(2)}_{\Psi \Psi} \Psi \Psi   -\frac{k^2}{a^2} C^{(2)}_{\Psi \pi} \Psi \pi 
\nonumber  \\& 
  +C_{\pi \pi} \pi \pi +C_{\pi \dot{\Phi}} \pi \dot{\Phi}+ C_{\pi \dot{\Psi}} \pi \dot{\Psi}+ C_{\pi \dot{\pi}} \pi \dot{\pi} -\frac{k^2}{a^2} a^{(2)}_{\pi \Phi} \pi \Phi  -\frac{k^2}{a^2} a^{(2)}_{\pi \Psi} \pi \Psi   -\frac{k^2}{a^2} a^{(2)}_{\pi \pi} \pi \pi 
\nonumber   \\& 
+C_{\dot{\Phi} \dot{\Phi}} \dot{\Phi} \dot{\Phi}+ C_{\dot{\Phi} \dot{\Psi}} \dot{\Phi} \dot{\Psi}+ C_{\dot{\Phi} \dot{\pi}} \dot{\Phi} \dot{\pi}  -\frac{k^2}{C^2} C^{(2)}_{\dot{\Phi} \Phi} \dot{\Phi} \Phi  -\frac{k^2}{C^2} C^{(2)}_{\dot{\Phi} \Psi} \dot{\Phi} \Psi   -\frac{k^2}{C^2} C^{(2)}_{\dot{\Phi} \pi} \dot{\Phi} \pi 
\nonumber   \\&
+ C_{ \dot{\Psi} \dot{\Psi}} \dot{\Psi} \dot{\Psi}+ C_{ \dot{\Psi}\dot{\pi}}  \dot{\Psi}\dot{\pi}  -\frac{k^2}{C^2} C^{(2)}_{\dot{\Psi} \Phi} \dot{\Psi} \Phi  -\frac{k^2}{C^2} C^{(2)}_{\dot{\Psi} \Psi} \dot{\Psi} \Psi   -\frac{k^2}{C^2} C^{(2)}_{\dot{\Psi} \pi} \dot{\Psi} \pi 
\nonumber   \\& 
  +C_{ \dot{\pi}\dot{\pi}}  \dot{\pi}\dot{\pi}  -\frac{k^2}{C^2} C^{(2)}_{\dot{\pi} \Phi} \dot{\pi} \Phi  -\frac{k^2}{C^2} C^{(2)}_{\dot{\pi} \Psi} \dot{\pi} \Psi   -\frac{k^2}{C^2} C^{(2)}_{\dot{\pi} \pi} \dot{\pi} \pi \text{ .}
\end{align}
Where;
\be
C_{\Phi \Phi}= \text{ .}
\ee
\be
C_{\Phi \Psi}=  \text{ .}
\ee
\be
C_{\Phi \pi}= \text{ .}
\ee
\be
C_{\Phi \dot{\Phi}}=  \text{ .}
\ee
\be
C_{\Phi \dot{\Psi}}= \text{ .}
\ee
\be
C_{\Phi \dot{\pi}}= \text{ .}
\ee
\be
C^{(2)}_{\Phi \Phi}=  \text{ .}
\ee
\be
C^{(2)}_{\Phi \Psi}=  \text{ .}
\ee
\be
C^{(2)}_{\Phi \pi}=  \text{ .}
\ee
\be
C_{\Psi \Psi}=    \text{ .}
\ee
\be
C_{\Psi \pi}=   \text{ .}
\ee
\be
C_{\Psi \dot{\Phi}}= \text{ .}
\ee
\be
C_{\Psi \dot{\Psi}}=   \text{ .}
\ee
\be
C_{\Psi \dot{\pi}}=   \text{ .}
\ee
\be
C^{(2)}_{\Psi \Phi}=  \text{ .}
\ee
\be
C^{(2)}_{\Psi \Psi}=  \text{ .}
\ee
\be
C^{(2)}_{\Psi \pi}= \text{ .}
\ee
\be
C_{\pi \pi}=  \text{ .}
\ee
\be
C_{\pi \dot{\Phi}}=  \text{ .}
\ee
\be
C_{\pi \dot{\Psi}}=   \text{ .}
\ee
\be
C_{\pi \dot{\pi}}=   \text{ .}
\ee
\be
C^{(2)}_{\pi \Phi}= \text{ .}
\ee
\be
C^{(2)}_{\pi \Psi}=  \text{ .}
\ee
\be
C^{(2)}_{\pi \pi}=  \text{ .}
\ee
\be
C_{\dot{\Phi} \dot{\Phi}}= \text{ .}
\ee
\be
C_{\dot{\Phi} \dot{\Psi}}=\text{ .}
\ee
\be
C_{\dot{\Phi} \dot{\pi}}=\text{ .}
\ee
\be
C^{(2)}_{\dot{\Phi} \Phi}= \text{ .}
\ee
\be
C^{(2)}_{\dot{\Phi} \Psi}= \text{ .}
\ee
\be
C^{(2)}_{\dot{\Phi} \pi}= \text{ .}
\ee
\be
C_{\dot{\Psi} \dot{\Psi}}= \text{ .}
\ee
\be
C_{\dot{\Psi} \dot{\pi}}= \text{ .}
\ee
\be
C^{(2)}_{\dot{\Psi} \Phi}= \text{ .}
\ee
\be
C^{(2)}_{\dot{\Psi} \Psi}= \text{ .}
\ee
\be
C^{(2)}_{\dot{\Psi} \pi}= \text{ .}
\ee
\be
C_{\dot{\pi} \dot{\pi}}=  \text{ .}
\ee
\be
C^{(2)}_{\dot{\pi} \Phi}=  \text{ .}
\ee
\be
C^{(2)}_{\dot{\pi} \Psi}= \text{ .}
\ee
\be
C^{(2)}_{\dot{\pi} \pi}= \text{ .}
\ee